update the generated files
git-svn-id: https://projects.brucker.ch/hol-testgen/svn/HOL-TestGen/trunk/hol-testgen@11418 3260e6d1-4efc-4170-b0a7-36055960796d

doc/Employee_AnalysisModel_UMLPart_generated.thy
@@ -2764,7 +2764,7 @@ definition "select\<^sub>P\<^sub>l\<^sub>a\<^sub>n\<^sub>e\<^sub>t\<O>\<U>\<T>\<
     | (mkoid\<^sub>P\<^sub>l\<^sub>a\<^sub>n\<^sub>e\<^sub>t ((mk\<^sub>P\<^sub>l\<^sub>a\<^sub>n\<^sub>e\<^sub>t_\<^sub>P\<^sub>e\<^sub>r\<^sub>s\<^sub>o\<^sub>n (person))) (_) (_)) \<Rightarrow> (select\<^sub>P\<^sub>e\<^sub>r\<^sub>s\<^sub>o\<^sub>n\<O>\<U>\<T>\<E>\<R>095\<W>\<O>\<R>\<L>\<D> (f) (person)))"
 
 (* 114 ************************************ 679 + 1 *)
-definition "select\<^sub>P\<^sub>e\<^sub>r\<^sub>s\<^sub>o\<^sub>n\<B>\<O>\<S>\<S> f = (select_object (mtSet) (UML_Set.OclIncluding) (UML_Set.OclANY) (f))"
+definition "select\<^sub>P\<^sub>e\<^sub>r\<^sub>s\<^sub>o\<^sub>n\<B>\<O>\<S>\<S> = select_object_any\<^sub>S\<^sub>e\<^sub>t"
 
 (* 115 ************************************ 680 + 14 *)
 consts dot_0_\<B>\<O>\<S>\<S> :: "(\<AA>, '\<alpha>) val \<Rightarrow> Person" ("(_) .boss")
@@ -3196,15 +3196,83 @@ lemma defined_mono_dot\<^sub>P\<^sub>l\<^sub>a\<^sub>n\<^sub>e\<^sub>t\<O>\<U>\<
   apply(case_tac "\<tau> \<Turnstile> (X \<triangleq> null)", insert StrongEq_L_subst2[where P = "(\<lambda>x. (\<delta> (x .outer_world@pre)))" and \<tau> = "\<tau>" and x = "X" and y = "null"], simp add: foundation16' dot\<^sub>P\<^sub>l\<^sub>a\<^sub>n\<^sub>e\<^sub>t\<O>\<U>\<T>\<E>\<R>095\<W>\<O>\<R>\<L>\<D>at_pre_null)
 by(simp add: defined_split)
 
-(* 126 ************************************ 850 + 0 *)
+(* 126 ************************************ 850 + 2 *)
+lemma is_repr_dot\<^sub>P\<^sub>e\<^sub>r\<^sub>s\<^sub>o\<^sub>n_0_\<B>\<O>\<S>\<S> : 
+assumes def_dot: "\<tau> \<Turnstile> (\<delta> ((X::Person) .boss))"
+shows "(is_represented_in_state (in_post_state) (X .boss) (Person) (\<tau>))"
+  apply(insert defined_mono_dot\<^sub>P\<^sub>e\<^sub>r\<^sub>s\<^sub>o\<^sub>n_0_\<B>\<O>\<S>\<S>[OF def_dot, simplified foundation16])
+  apply(case_tac "(X (\<tau>))", simp add: bot_option_def)
+  proof - fix a0 show "(X (\<tau>)) \<noteq> null \<Longrightarrow> (X (\<tau>)) = (Some (a0)) \<Longrightarrow> ?thesis"
+  apply(case_tac "a0", simp add: null_option_def bot_option_def, clarify)
+  proof - fix a show "(X (\<tau>)) = (Some ((Some (a)))) \<Longrightarrow> ?thesis"
+  apply(case_tac "(heap ((in_post_state (\<tau>))) ((oid_of (a))))", simp add: invalid_def bot_option_def)
+  apply(insert def_dot, simp add: dot\<^sub>P\<^sub>e\<^sub>r\<^sub>s\<^sub>o\<^sub>n_0_\<B>\<O>\<S>\<S> is_represented_in_state_def select\<^sub>P\<^sub>e\<^sub>r\<^sub>s\<^sub>o\<^sub>n\<B>\<O>\<S>\<S>_def deref_oid\<^sub>P\<^sub>e\<^sub>r\<^sub>s\<^sub>o\<^sub>n_def in_post_state_def defined_def OclValid_def false_def true_def invalid_def bot_fun_def split: split_if_asm)
+  proof - fix b show "(X (\<tau>)) = (Some ((Some (a)))) \<Longrightarrow> (heap ((in_post_state (\<tau>))) ((oid_of (a)))) = (Some (b)) \<Longrightarrow> ?thesis"
+  apply(insert def_dot[simplified foundation16], auto simp: dot\<^sub>P\<^sub>e\<^sub>r\<^sub>s\<^sub>o\<^sub>n_0_\<B>\<O>\<S>\<S> is_represented_in_state_def deref_oid\<^sub>P\<^sub>e\<^sub>r\<^sub>s\<^sub>o\<^sub>n_def bot_option_def null_option_def)
+  apply(case_tac "b", simp_all add: invalid_def bot_option_def)
+  apply(simp add: deref_assocs\<^sub>P\<^sub>e\<^sub>r\<^sub>s\<^sub>o\<^sub>n_0_\<B>\<O>\<S>\<S>_def deref_assocs_def)
+  apply(case_tac "(assocs ((in_post_state (\<tau>))) (oid\<^sub>P\<^sub>e\<^sub>r\<^sub>s\<^sub>o\<^sub>n_0_\<B>\<O>\<S>\<S>))", simp add: invalid_def bot_option_def, simp add: select\<^sub>P\<^sub>e\<^sub>r\<^sub>s\<^sub>o\<^sub>n\<B>\<O>\<S>\<S>_def)
+  proof - fix r typeoid          let ?t = "(Some ((Some (r)))) \<in> (Some o OclAsType\<^sub>P\<^sub>e\<^sub>r\<^sub>s\<^sub>o\<^sub>n_\<AA>) ` (ran ((heap ((in_post_state (\<tau>))))))"
+          let ?sel_any = "(select_object_any\<^sub>S\<^sub>e\<^sub>t ((deref_oid\<^sub>P\<^sub>e\<^sub>r\<^sub>s\<^sub>o\<^sub>n (in_post_state) (reconst_basetype))))" show "((?sel_any) (typeoid) (\<tau>)) = (Some ((Some (r)))) \<Longrightarrow> ?t"
+  proof - fix aa show "\<tau> \<Turnstile> (\<delta> (((?sel_any) (aa)))) \<Longrightarrow> ((?sel_any) (aa) (\<tau>)) = (Some ((Some (r)))) \<Longrightarrow> ?t"
+  apply(drule select_object_any_exec\<^sub>S\<^sub>e\<^sub>t[simplified foundation22], erule exE)
+  proof - fix e show "((?sel_any) (aa) (\<tau>)) = (Some ((Some (r)))) \<Longrightarrow> ((?sel_any) (aa) (\<tau>)) = (deref_oid\<^sub>P\<^sub>e\<^sub>r\<^sub>s\<^sub>o\<^sub>n (in_post_state) (reconst_basetype) (e) (\<tau>)) \<Longrightarrow> ?t"
+  apply(simp add: deref_oid\<^sub>P\<^sub>e\<^sub>r\<^sub>s\<^sub>o\<^sub>n_def)
+  apply(case_tac "(heap ((in_post_state (\<tau>))) (e))", simp add: invalid_def bot_option_def, simp)
+  proof - fix aaa show "(case aaa of (in\<^sub>P\<^sub>e\<^sub>r\<^sub>s\<^sub>o\<^sub>n (obj)) \<Rightarrow> (reconst_basetype (obj) (\<tau>))
+    | _ \<Rightarrow> (invalid (\<tau>))) = (Some ((Some (r)))) \<Longrightarrow> (heap ((in_post_state (\<tau>))) (e)) = (Some (aaa)) \<Longrightarrow> ?t"
+  apply(case_tac "aaa", auto simp: invalid_def bot_option_def image_def ran_def)
+  apply(rule exI[where x = "(in\<^sub>P\<^sub>e\<^sub>r\<^sub>s\<^sub>o\<^sub>n (r))"], simp add: OclAsType\<^sub>P\<^sub>e\<^sub>r\<^sub>s\<^sub>o\<^sub>n_\<AA>_def Let_def reconst_basetype_def split: split_if_asm)
+by(rule) qed 
+  apply_end((blast)+)
+ qed 
+  apply_end(simp_all only: )
+  apply_end(simp add: foundation16 bot_option_def null_option_def)
+ qed qed qed qed 
+  apply_end(simp_all)
+ qed
+lemma is_repr_dot\<^sub>P\<^sub>e\<^sub>r\<^sub>s\<^sub>o\<^sub>n_0_\<B>\<O>\<S>\<S>at_pre : 
+assumes def_dot: "\<tau> \<Turnstile> (\<delta> ((X::Person) .boss@pre))"
+shows "(is_represented_in_state (in_pre_state) (X .boss@pre) (Person) (\<tau>))"
+  apply(insert defined_mono_dot\<^sub>P\<^sub>e\<^sub>r\<^sub>s\<^sub>o\<^sub>n_0_\<B>\<O>\<S>\<S>at_pre[OF def_dot, simplified foundation16])
+  apply(case_tac "(X (\<tau>))", simp add: bot_option_def)
+  proof - fix a0 show "(X (\<tau>)) \<noteq> null \<Longrightarrow> (X (\<tau>)) = (Some (a0)) \<Longrightarrow> ?thesis"
+  apply(case_tac "a0", simp add: null_option_def bot_option_def, clarify)
+  proof - fix a show "(X (\<tau>)) = (Some ((Some (a)))) \<Longrightarrow> ?thesis"
+  apply(case_tac "(heap ((in_pre_state (\<tau>))) ((oid_of (a))))", simp add: invalid_def bot_option_def)
+  apply(insert def_dot, simp add: dot\<^sub>P\<^sub>e\<^sub>r\<^sub>s\<^sub>o\<^sub>n_0_\<B>\<O>\<S>\<S>at_pre is_represented_in_state_def select\<^sub>P\<^sub>e\<^sub>r\<^sub>s\<^sub>o\<^sub>n\<B>\<O>\<S>\<S>_def deref_oid\<^sub>P\<^sub>e\<^sub>r\<^sub>s\<^sub>o\<^sub>n_def in_pre_state_def defined_def OclValid_def false_def true_def invalid_def bot_fun_def split: split_if_asm)
+  proof - fix b show "(X (\<tau>)) = (Some ((Some (a)))) \<Longrightarrow> (heap ((in_pre_state (\<tau>))) ((oid_of (a)))) = (Some (b)) \<Longrightarrow> ?thesis"
+  apply(insert def_dot[simplified foundation16], auto simp: dot\<^sub>P\<^sub>e\<^sub>r\<^sub>s\<^sub>o\<^sub>n_0_\<B>\<O>\<S>\<S>at_pre is_represented_in_state_def deref_oid\<^sub>P\<^sub>e\<^sub>r\<^sub>s\<^sub>o\<^sub>n_def bot_option_def null_option_def)
+  apply(case_tac "b", simp_all add: invalid_def bot_option_def)
+  apply(simp add: deref_assocs\<^sub>P\<^sub>e\<^sub>r\<^sub>s\<^sub>o\<^sub>n_0_\<B>\<O>\<S>\<S>_def deref_assocs_def)
+  apply(case_tac "(assocs ((in_pre_state (\<tau>))) (oid\<^sub>P\<^sub>e\<^sub>r\<^sub>s\<^sub>o\<^sub>n_0_\<B>\<O>\<S>\<S>))", simp add: invalid_def bot_option_def, simp add: select\<^sub>P\<^sub>e\<^sub>r\<^sub>s\<^sub>o\<^sub>n\<B>\<O>\<S>\<S>_def)
+  proof - fix r typeoid          let ?t = "(Some ((Some (r)))) \<in> (Some o OclAsType\<^sub>P\<^sub>e\<^sub>r\<^sub>s\<^sub>o\<^sub>n_\<AA>) ` (ran ((heap ((in_pre_state (\<tau>))))))"
+          let ?sel_any = "(select_object_any\<^sub>S\<^sub>e\<^sub>t ((deref_oid\<^sub>P\<^sub>e\<^sub>r\<^sub>s\<^sub>o\<^sub>n (in_pre_state) (reconst_basetype))))" show "((?sel_any) (typeoid) (\<tau>)) = (Some ((Some (r)))) \<Longrightarrow> ?t"
+  proof - fix aa show "\<tau> \<Turnstile> (\<delta> (((?sel_any) (aa)))) \<Longrightarrow> ((?sel_any) (aa) (\<tau>)) = (Some ((Some (r)))) \<Longrightarrow> ?t"
+  apply(drule select_object_any_exec\<^sub>S\<^sub>e\<^sub>t[simplified foundation22], erule exE)
+  proof - fix e show "((?sel_any) (aa) (\<tau>)) = (Some ((Some (r)))) \<Longrightarrow> ((?sel_any) (aa) (\<tau>)) = (deref_oid\<^sub>P\<^sub>e\<^sub>r\<^sub>s\<^sub>o\<^sub>n (in_pre_state) (reconst_basetype) (e) (\<tau>)) \<Longrightarrow> ?t"
+  apply(simp add: deref_oid\<^sub>P\<^sub>e\<^sub>r\<^sub>s\<^sub>o\<^sub>n_def)
+  apply(case_tac "(heap ((in_pre_state (\<tau>))) (e))", simp add: invalid_def bot_option_def, simp)
+  proof - fix aaa show "(case aaa of (in\<^sub>P\<^sub>e\<^sub>r\<^sub>s\<^sub>o\<^sub>n (obj)) \<Rightarrow> (reconst_basetype (obj) (\<tau>))
+    | _ \<Rightarrow> (invalid (\<tau>))) = (Some ((Some (r)))) \<Longrightarrow> (heap ((in_pre_state (\<tau>))) (e)) = (Some (aaa)) \<Longrightarrow> ?t"
+  apply(case_tac "aaa", auto simp: invalid_def bot_option_def image_def ran_def)
+  apply(rule exI[where x = "(in\<^sub>P\<^sub>e\<^sub>r\<^sub>s\<^sub>o\<^sub>n (r))"], simp add: OclAsType\<^sub>P\<^sub>e\<^sub>r\<^sub>s\<^sub>o\<^sub>n_\<AA>_def Let_def reconst_basetype_def split: split_if_asm)
+by(rule) qed 
+  apply_end((blast)+)
+ qed 
+  apply_end(simp_all only: )
+  apply_end(simp add: foundation16 bot_option_def null_option_def)
+ qed qed qed qed 
+  apply_end(simp_all)
+ qed
 
-(* 127 ************************************ 850 + 1 *)
+(* 127 ************************************ 852 + 1 *)
 section{* A Little Infra-structure on Example States *}
 
-(* 128 ************************************ 851 + 1 *)
+(* 128 ************************************ 853 + 1 *)
 text{*  *}
 
-(* 129 ************************************ 852 + 1 *)
+(* 129 ************************************ 854 + 1 *)
 text{* 
 
 The example we are defining in this section comes from the figure~\ref{fig:eam1_system-states}.
@@ -3216,11 +3284,11 @@ The example we are defining in this section comes from the figure~\ref{fig:eam1_
 \end{figure}
  *}
 
-(* 130 ************************************ 853 + 1 *)
+(* 130 ************************************ 855 + 1 *)
 lemmas [simp,code_unfold] = state.defs
                             const_ss
 
-(* 131 ************************************ 854 + 1 *)
+(* 131 ************************************ 856 + 1 *)
 lemmas[simp,code_unfold] = OclAsType\<^sub>P\<^sub>e\<^sub>r\<^sub>s\<^sub>o\<^sub>n_Planet
                             OclAsType\<^sub>P\<^sub>e\<^sub>r\<^sub>s\<^sub>o\<^sub>n_Galaxy
                             OclAsType\<^sub>P\<^sub>e\<^sub>r\<^sub>s\<^sub>o\<^sub>n_OclAny
@@ -3234,7 +3302,7 @@ lemmas[simp,code_unfold] = OclAsType\<^sub>P\<^sub>e\<^sub>r\<^sub>s\<^sub>o\<^s
                             OclAsType\<^sub>O\<^sub>c\<^sub>l\<^sub>A\<^sub>n\<^sub>y_Planet
                             OclAsType\<^sub>O\<^sub>c\<^sub>l\<^sub>A\<^sub>n\<^sub>y_Galaxy
 
-(* 132 ************************************ 855 + 11 *)
+(* 132 ************************************ 857 + 11 *)
 definition "oid1 = 1"
 definition "oid2 = 2"
 definition "oid3 = 3"
@@ -3247,7 +3315,7 @@ definition "oid9 = 9"
 definition "oid10 = 10"
 definition "oid11 = 11"
 
-(* 133 ************************************ 866 + 22 *)
+(* 133 ************************************ 868 + 22 *)
 definition "X\<^sub>P\<^sub>e\<^sub>r\<^sub>s\<^sub>o\<^sub>n1\<^sub>P\<^sub>e\<^sub>r\<^sub>s\<^sub>o\<^sub>n = (mkoid\<^sub>P\<^sub>e\<^sub>r\<^sub>s\<^sub>o\<^sub>n ((mk\<^sub>P\<^sub>e\<^sub>r\<^sub>s\<^sub>o\<^sub>n (oid1) (None) (None) (None) (None) (None))) (\<lfloor>1300\<rfloor>))"
 definition "X\<^sub>P\<^sub>e\<^sub>r\<^sub>s\<^sub>o\<^sub>n2\<^sub>P\<^sub>e\<^sub>r\<^sub>s\<^sub>o\<^sub>n = (mkoid\<^sub>P\<^sub>e\<^sub>r\<^sub>s\<^sub>o\<^sub>n ((mk\<^sub>P\<^sub>e\<^sub>r\<^sub>s\<^sub>o\<^sub>n (oid2) (None) (None) (None) (None) (None))) (\<lfloor>1800\<rfloor>))"
 definition "X\<^sub>P\<^sub>e\<^sub>r\<^sub>s\<^sub>o\<^sub>n3\<^sub>P\<^sub>e\<^sub>r\<^sub>s\<^sub>o\<^sub>n = (mkoid\<^sub>P\<^sub>e\<^sub>r\<^sub>s\<^sub>o\<^sub>n ((mk\<^sub>P\<^sub>e\<^sub>r\<^sub>s\<^sub>o\<^sub>n (oid3) (None) (None) (None) (None) (None))) (None))"
@@ -3271,25 +3339,25 @@ definition "(X\<^sub>P\<^sub>e\<^sub>r\<^sub>s\<^sub>o\<^sub>n9::Person) = (\<la
 definition "(X0::Person) = (\<lambda>_. \<lfloor>\<lfloor>X0\<^sub>P\<^sub>e\<^sub>r\<^sub>s\<^sub>o\<^sub>n\<rfloor>\<rfloor>)"
 definition "(P1::Planet) = (\<lambda>_. \<lfloor>\<lfloor>P1\<^sub>P\<^sub>l\<^sub>a\<^sub>n\<^sub>e\<^sub>t\<rfloor>\<rfloor>)"
 
-(* 134 ************************************ 888 + 1 *)
+(* 134 ************************************ 890 + 1 *)
 ML{* (Ty'.check ([(OCL.Writeln , "X\<^sub>P\<^sub>e\<^sub>r\<^sub>s\<^sub>o\<^sub>n1 .boss = Set{ X\<^sub>P\<^sub>e\<^sub>r\<^sub>s\<^sub>o\<^sub>n2 }") , (OCL.Writeln , "X\<^sub>P\<^sub>e\<^sub>r\<^sub>s\<^sub>o\<^sub>n1 /* unnamed attribute */ = Set{}") , (OCL.Writeln , "X\<^sub>P\<^sub>e\<^sub>r\<^sub>s\<^sub>o\<^sub>n2 .boss = Set{ X\<^sub>P\<^sub>e\<^sub>r\<^sub>s\<^sub>o\<^sub>n2 }") , (OCL.Writeln , "X\<^sub>P\<^sub>e\<^sub>r\<^sub>s\<^sub>o\<^sub>n2 /* unnamed attribute */ = Set{ X\<^sub>P\<^sub>e\<^sub>r\<^sub>s\<^sub>o\<^sub>n1 , X\<^sub>P\<^sub>e\<^sub>r\<^sub>s\<^sub>o\<^sub>n2 }") , (OCL.Writeln , "X\<^sub>P\<^sub>e\<^sub>r\<^sub>s\<^sub>o\<^sub>n3 .boss = Set{}") , (OCL.Writeln , "X\<^sub>P\<^sub>e\<^sub>r\<^sub>s\<^sub>o\<^sub>n3 /* unnamed attribute */ = Set{}") , (OCL.Writeln , "X\<^sub>P\<^sub>e\<^sub>r\<^sub>s\<^sub>o\<^sub>n4 .boss = Set{}") , (OCL.Writeln , "X\<^sub>P\<^sub>e\<^sub>r\<^sub>s\<^sub>o\<^sub>n4 /* unnamed attribute */ = Set{}") , (OCL.Writeln , "X\<^sub>P\<^sub>e\<^sub>r\<^sub>s\<^sub>o\<^sub>n5 .boss = Set{}") , (OCL.Writeln , "X\<^sub>P\<^sub>e\<^sub>r\<^sub>s\<^sub>o\<^sub>n5 /* unnamed attribute */ = Set{}") , (OCL.Writeln , "X\<^sub>P\<^sub>e\<^sub>r\<^sub>s\<^sub>o\<^sub>n6 .boss = Set{ X\<^sub>P\<^sub>e\<^sub>r\<^sub>s\<^sub>o\<^sub>n7 }") , (OCL.Writeln , "X\<^sub>P\<^sub>e\<^sub>r\<^sub>s\<^sub>o\<^sub>n6 /* unnamed attribute */ = Set{}") , (OCL.Writeln , "X\<^sub>P\<^sub>e\<^sub>r\<^sub>s\<^sub>o\<^sub>n7 .boss = Set{ X\<^sub>P\<^sub>e\<^sub>r\<^sub>s\<^sub>o\<^sub>n7 }") , (OCL.Writeln , "X\<^sub>P\<^sub>e\<^sub>r\<^sub>s\<^sub>o\<^sub>n7 /* unnamed attribute */ = Set{ X\<^sub>P\<^sub>e\<^sub>r\<^sub>s\<^sub>o\<^sub>n6 , X\<^sub>P\<^sub>e\<^sub>r\<^sub>s\<^sub>o\<^sub>n7 }") , (OCL.Writeln , "X\<^sub>P\<^sub>e\<^sub>r\<^sub>s\<^sub>o\<^sub>n9 .boss = Set{}") , (OCL.Writeln , "X\<^sub>P\<^sub>e\<^sub>r\<^sub>s\<^sub>o\<^sub>n9 /* unnamed attribute */ = Set{}") , (OCL.Writeln , "X0 .boss = Set{}") , (OCL.Writeln , "X0 /* unnamed attribute */ = Set{}")]) (" error(s)")) *}
 
-(* 135 ************************************ 889 + 4 *)
+(* 135 ************************************ 891 + 4 *)
 generation_syntax [ shallow (generation_semantics [ analysis ]) ]
 setup{* (Generation_mode.update_compiler_config ((K (let open OCL in Ocl_compiler_config_ext (true, NONE, Oids ((Code_Numeral.Nat 0), (Code_Numeral.Nat 1), (Code_Numeral.Nat 12)), I ((Code_Numeral.Nat 0), (Code_Numeral.Nat 0)), Gen_only_analysis, SOME (OclClass ((OCL.SS_base (OCL.ST "OclAny")), nil, uncurry cons (OclClass ((OCL.SS_base (OCL.ST "Galaxy")), uncurry cons (I ((OCL.SS_base (OCL.ST "sound")), OclTy_base_void), uncurry cons (I ((OCL.SS_base (OCL.ST "moving")), OclTy_base_boolean), uncurry cons (I ((OCL.SS_base (OCL.ST "outer_world")), OclTy_collection (Ocl_multiplicity_ext (nil, NONE, uncurry cons (Set, nil), ()), OclTy_collection (Ocl_multiplicity_ext (nil, NONE, uncurry cons (Sequence, nil), ()), OclTy_object (OclTyObj (OclTyCore_pre ((OCL.SS_base (OCL.ST "Planet"))), nil))))), nil))), uncurry cons (OclClass ((OCL.SS_base (OCL.ST "Planet")), uncurry cons (I ((OCL.SS_base (OCL.ST "wormhole")), OclTy_base_unlimitednatural), uncurry cons (I ((OCL.SS_base (OCL.ST "weight")), OclTy_base_integer), nil)), uncurry cons (OclClass ((OCL.SS_base (OCL.ST "Person")), uncurry cons (I ((OCL.SS_base (OCL.ST "boss")), OclTy_object (OclTyObj (OclTyCore (Ocl_ty_class_ext ((OCL.SS_base (OCL.ST "oid")), (Code_Numeral.Nat 0), (Code_Numeral.Nat 2), Ocl_ty_class_node_ext ((Code_Numeral.Nat 0), Ocl_multiplicity_ext (uncurry cons (I (Mult_star, NONE), nil), NONE, nil, ()), (OCL.SS_base (OCL.ST "Person")), ()), Ocl_ty_class_node_ext ((Code_Numeral.Nat 1), Ocl_multiplicity_ext (uncurry cons (I (Mult_nat ((Code_Numeral.Nat 0)), SOME (Mult_nat ((Code_Numeral.Nat 1)))), nil), SOME ((OCL.SS_base (OCL.ST "boss"))), nil, ()), (OCL.SS_base (OCL.ST "Person")), ()), ())), nil))), uncurry cons (I ((OCL.SS_base (OCL.ST "salary")), OclTy_base_integer), nil)), nil), nil)), nil)), nil))), uncurry cons (OclAstInstance (OclInstance (uncurry cons (Ocl_instance_single_ext (SOME ((OCL.SS_base (OCL.ST "X\<^sub>P\<^sub>e\<^sub>r\<^sub>s\<^sub>o\<^sub>n1"))), (OCL.SS_base (OCL.ST "Person")), OclAttrNoCast (uncurry cons (I ((OCL.SS_base (OCL.ST "salary")), ShallB_term (OclDefInteger ((OCL.SS_base (OCL.ST "1300"))))), uncurry cons (I ((OCL.SS_base (OCL.ST "boss")), ShallB_str ((OCL.SS_base (OCL.ST "X\<^sub>P\<^sub>e\<^sub>r\<^sub>s\<^sub>o\<^sub>n2")))), nil))), ()), uncurry cons (Ocl_instance_single_ext (SOME ((OCL.SS_base (OCL.ST "X\<^sub>P\<^sub>e\<^sub>r\<^sub>s\<^sub>o\<^sub>n2"))), (OCL.SS_base (OCL.ST "Person")), OclAttrNoCast (uncurry cons (I ((OCL.SS_base (OCL.ST "salary")), ShallB_term (OclDefInteger ((OCL.SS_base (OCL.ST "1800"))))), uncurry cons (I ((OCL.SS_base (OCL.ST "boss")), ShallB_str ((OCL.SS_base (OCL.ST "X\<^sub>P\<^sub>e\<^sub>r\<^sub>s\<^sub>o\<^sub>n2")))), nil))), ()), uncurry cons (Ocl_instance_single_ext (SOME ((OCL.SS_base (OCL.ST "X\<^sub>P\<^sub>e\<^sub>r\<^sub>s\<^sub>o\<^sub>n3"))), (OCL.SS_base (OCL.ST "Person")), OclAttrNoCast (nil), ()), uncurry cons (Ocl_instance_single_ext (SOME ((OCL.SS_base (OCL.ST "X\<^sub>P\<^sub>e\<^sub>r\<^sub>s\<^sub>o\<^sub>n4"))), (OCL.SS_base (OCL.ST "Person")), OclAttrNoCast (uncurry cons (I ((OCL.SS_base (OCL.ST "salary")), ShallB_term (OclDefInteger ((OCL.SS_base (OCL.ST "2900"))))), nil)), ()), uncurry cons (Ocl_instance_single_ext (SOME ((OCL.SS_base (OCL.ST "X\<^sub>P\<^sub>e\<^sub>r\<^sub>s\<^sub>o\<^sub>n5"))), (OCL.SS_base (OCL.ST "Person")), OclAttrNoCast (uncurry cons (I ((OCL.SS_base (OCL.ST "salary")), ShallB_term (OclDefInteger ((OCL.SS_base (OCL.ST "3500"))))), nil)), ()), uncurry cons (Ocl_instance_single_ext (SOME ((OCL.SS_base (OCL.ST "X\<^sub>P\<^sub>e\<^sub>r\<^sub>s\<^sub>o\<^sub>n6"))), (OCL.SS_base (OCL.ST "Person")), OclAttrNoCast (uncurry cons (I ((OCL.SS_base (OCL.ST "salary")), ShallB_term (OclDefInteger ((OCL.SS_base (OCL.ST "2500"))))), uncurry cons (I ((OCL.SS_base (OCL.ST "boss")), ShallB_str ((OCL.SS_base (OCL.ST "X\<^sub>P\<^sub>e\<^sub>r\<^sub>s\<^sub>o\<^sub>n7")))), nil))), ()), uncurry cons (Ocl_instance_single_ext (SOME ((OCL.SS_base (OCL.ST "X\<^sub>P\<^sub>e\<^sub>r\<^sub>s\<^sub>o\<^sub>n7"))), (OCL.SS_base (OCL.ST "OclAny")), OclAttrCast ((OCL.SS_base (OCL.ST "Person")), OclAttrNoCast (uncurry cons (I ((OCL.SS_base (OCL.ST "salary")), ShallB_term (OclDefInteger ((OCL.SS_base (OCL.ST "3200"))))), uncurry cons (I ((OCL.SS_base (OCL.ST "boss")), ShallB_str ((OCL.SS_base (OCL.ST "X\<^sub>P\<^sub>e\<^sub>r\<^sub>s\<^sub>o\<^sub>n7")))), nil))), nil), ()), uncurry cons (Ocl_instance_single_ext (SOME ((OCL.SS_base (OCL.ST "X\<^sub>P\<^sub>e\<^sub>r\<^sub>s\<^sub>o\<^sub>n8"))), (OCL.SS_base (OCL.ST "OclAny")), OclAttrNoCast (nil), ()), uncurry cons (Ocl_instance_single_ext (SOME ((OCL.SS_base (OCL.ST "X\<^sub>P\<^sub>e\<^sub>r\<^sub>s\<^sub>o\<^sub>n9"))), (OCL.SS_base (OCL.ST "Person")), OclAttrNoCast (uncurry cons (I ((OCL.SS_base (OCL.ST "salary")), ShallB_term (OclDefInteger ((OCL.SS_base (OCL.ST "0"))))), nil)), ()), uncurry cons (Ocl_instance_single_ext (SOME ((OCL.SS_base (OCL.ST "X0"))), (OCL.SS_base (OCL.ST "Person")), OclAttrNoCast (uncurry cons (I ((OCL.SS_base (OCL.ST "outer_world")), ShallB_list (uncurry cons (ShallB_list (uncurry cons (ShallB_str ((OCL.SS_base (OCL.ST "P1"))), nil)), nil))), nil)), ()), uncurry cons (Ocl_instance_single_ext (SOME ((OCL.SS_base (OCL.ST "P1"))), (OCL.SS_base (OCL.ST "Planet")), OclAttrNoCast (uncurry cons (I ((OCL.SS_base (OCL.ST "outer_world")), ShallB_list (uncurry cons (ShallB_list (uncurry cons (ShallB_str ((OCL.SS_base (OCL.ST "P1"))), nil)), uncurry cons (ShallB_list (uncurry cons (ShallB_self (Oid ((Code_Numeral.Nat 10))), nil)), nil)))), nil)), ()), nil))))))))))))), uncurry cons (OclAstClassRaw (Floor1, Ocl_class_raw_ext (OclTyObj (OclTyCore_pre ((OCL.SS_base (OCL.ST "Galaxy"))), nil), uncurry cons (I ((OCL.SS_base (OCL.ST "sound")), OclTy_base_void), uncurry cons (I ((OCL.SS_base (OCL.ST "moving")), OclTy_base_boolean), uncurry cons (I ((OCL.SS_base (OCL.ST "outer_world")), OclTy_collection (Ocl_multiplicity_ext (nil, NONE, uncurry cons (Set, nil), ()), OclTy_binding (I (NONE, OclTy_collection (Ocl_multiplicity_ext (nil, NONE, uncurry cons (Sequence, nil), ()), OclTy_binding (I (NONE, OclTy_object (OclTyObj (OclTyCore_pre ((OCL.SS_base (OCL.ST "Planet"))), nil))))))))), nil))), nil, false, ())), uncurry cons (OclAstClassRaw (Floor1, Ocl_class_raw_ext (OclTyObj (OclTyCore_pre ((OCL.SS_base (OCL.ST "Planet"))), uncurry cons (uncurry cons (OclTyCore_pre ((OCL.SS_base (OCL.ST "Galaxy"))), nil), nil)), uncurry cons (I ((OCL.SS_base (OCL.ST "wormhole")), OclTy_base_unlimitednatural), uncurry cons (I ((OCL.SS_base (OCL.ST "weight")), OclTy_base_integer), nil)), nil, false, ())), uncurry cons (OclAstAssociation (Ocl_association_ext (OclAssTy_association, OclAssRel (uncurry cons (I (OclTyObj (OclTyCore_pre ((OCL.SS_base (OCL.ST "Person"))), nil), Ocl_multiplicity_ext (uncurry cons (I (Mult_star, NONE), nil), NONE, nil, ())), uncurry cons (I (OclTyObj (OclTyCore_pre ((OCL.SS_base (OCL.ST "Person"))), nil), Ocl_multiplicity_ext (uncurry cons (I (Mult_nat ((Code_Numeral.Nat 0)), SOME (Mult_nat ((Code_Numeral.Nat 1)))), nil), SOME ((OCL.SS_base (OCL.ST "boss"))), nil, ())), nil))), ())), uncurry cons (OclAstClassRaw (Floor1, Ocl_class_raw_ext (OclTyObj (OclTyCore_pre ((OCL.SS_base (OCL.ST "Person"))), uncurry cons (uncurry cons (OclTyCore_pre ((OCL.SS_base (OCL.ST "Planet"))), nil), nil)), uncurry cons (I ((OCL.SS_base (OCL.ST "salary")), OclTy_base_integer), nil), nil, false, ())), nil))))), uncurry cons (I ((OCL.ST "P1"), I (Ocl_instance_single_ext (SOME ((OCL.SS_base (OCL.ST "P1"))), (OCL.SS_base (OCL.ST "Planet")), OclAttrNoCast (uncurry cons (I ((OCL.SS_base (OCL.ST "outer_world")), ShallB_list (uncurry cons (ShallB_list (uncurry cons (ShallB_str ((OCL.SS_base (OCL.ST "P1"))), nil)), uncurry cons (ShallB_list (uncurry cons (ShallB_self (Oid ((Code_Numeral.Nat 10))), nil)), nil)))), nil)), ()), Oids ((Code_Numeral.Nat 0), (Code_Numeral.Nat 1), (Code_Numeral.Nat 11)))), uncurry cons (I ((OCL.ST "X0"), I (Ocl_instance_single_ext (SOME ((OCL.SS_base (OCL.ST "X0"))), (OCL.SS_base (OCL.ST "Person")), OclAttrNoCast (uncurry cons (I ((OCL.SS_base (OCL.ST "outer_world")), ShallB_list (uncurry cons (ShallB_list (uncurry cons (ShallB_str ((OCL.SS_base (OCL.ST "P1"))), nil)), nil))), nil)), ()), Oids ((Code_Numeral.Nat 0), (Code_Numeral.Nat 1), (Code_Numeral.Nat 10)))), uncurry cons (I ((OCL.ST "X\<^sub>P\<^sub>e\<^sub>r\<^sub>s\<^sub>o\<^sub>n9"), I (Ocl_instance_single_ext (SOME ((OCL.SS_base (OCL.ST "X\<^sub>P\<^sub>e\<^sub>r\<^sub>s\<^sub>o\<^sub>n9"))), (OCL.SS_base (OCL.ST "Person")), OclAttrNoCast (uncurry cons (I ((OCL.SS_base (OCL.ST "salary")), ShallB_term (OclDefInteger ((OCL.SS_base (OCL.ST "0"))))), nil)), ()), Oids ((Code_Numeral.Nat 0), (Code_Numeral.Nat 1), (Code_Numeral.Nat 9)))), uncurry cons (I ((OCL.ST "X\<^sub>P\<^sub>e\<^sub>r\<^sub>s\<^sub>o\<^sub>n8"), I (Ocl_instance_single_ext (SOME ((OCL.SS_base (OCL.ST "X\<^sub>P\<^sub>e\<^sub>r\<^sub>s\<^sub>o\<^sub>n8"))), (OCL.SS_base (OCL.ST "OclAny")), OclAttrNoCast (nil), ()), Oids ((Code_Numeral.Nat 0), (Code_Numeral.Nat 1), (Code_Numeral.Nat 8)))), uncurry cons (I ((OCL.ST "X\<^sub>P\<^sub>e\<^sub>r\<^sub>s\<^sub>o\<^sub>n7"), I (Ocl_instance_single_ext (SOME ((OCL.SS_base (OCL.ST "X\<^sub>P\<^sub>e\<^sub>r\<^sub>s\<^sub>o\<^sub>n7"))), (OCL.SS_base (OCL.ST "OclAny")), OclAttrCast ((OCL.SS_base (OCL.ST "Person")), OclAttrNoCast (uncurry cons (I ((OCL.SS_base (OCL.ST "salary")), ShallB_term (OclDefInteger ((OCL.SS_base (OCL.ST "3200"))))), uncurry cons (I ((OCL.SS_base (OCL.ST "boss")), ShallB_str ((OCL.SS_base (OCL.ST "X\<^sub>P\<^sub>e\<^sub>r\<^sub>s\<^sub>o\<^sub>n7")))), nil))), nil), ()), Oids ((Code_Numeral.Nat 0), (Code_Numeral.Nat 1), (Code_Numeral.Nat 7)))), uncurry cons (I ((OCL.ST "X\<^sub>P\<^sub>e\<^sub>r\<^sub>s\<^sub>o\<^sub>n6"), I (Ocl_instance_single_ext (SOME ((OCL.SS_base (OCL.ST "X\<^sub>P\<^sub>e\<^sub>r\<^sub>s\<^sub>o\<^sub>n6"))), (OCL.SS_base (OCL.ST "Person")), OclAttrNoCast (uncurry cons (I ((OCL.SS_base (OCL.ST "salary")), ShallB_term (OclDefInteger ((OCL.SS_base (OCL.ST "2500"))))), uncurry cons (I ((OCL.SS_base (OCL.ST "boss")), ShallB_str ((OCL.SS_base (OCL.ST "X\<^sub>P\<^sub>e\<^sub>r\<^sub>s\<^sub>o\<^sub>n7")))), nil))), ()), Oids ((Code_Numeral.Nat 0), (Code_Numeral.Nat 1), (Code_Numeral.Nat 6)))), uncurry cons (I ((OCL.ST "X\<^sub>P\<^sub>e\<^sub>r\<^sub>s\<^sub>o\<^sub>n5"), I (Ocl_instance_single_ext (SOME ((OCL.SS_base (OCL.ST "X\<^sub>P\<^sub>e\<^sub>r\<^sub>s\<^sub>o\<^sub>n5"))), (OCL.SS_base (OCL.ST "Person")), OclAttrNoCast (uncurry cons (I ((OCL.SS_base (OCL.ST "salary")), ShallB_term (OclDefInteger ((OCL.SS_base (OCL.ST "3500"))))), nil)), ()), Oids ((Code_Numeral.Nat 0), (Code_Numeral.Nat 1), (Code_Numeral.Nat 5)))), uncurry cons (I ((OCL.ST "X\<^sub>P\<^sub>e\<^sub>r\<^sub>s\<^sub>o\<^sub>n4"), I (Ocl_instance_single_ext (SOME ((OCL.SS_base (OCL.ST "X\<^sub>P\<^sub>e\<^sub>r\<^sub>s\<^sub>o\<^sub>n4"))), (OCL.SS_base (OCL.ST "Person")), OclAttrNoCast (uncurry cons (I ((OCL.SS_base (OCL.ST "salary")), ShallB_term (OclDefInteger ((OCL.SS_base (OCL.ST "2900"))))), nil)), ()), Oids ((Code_Numeral.Nat 0), (Code_Numeral.Nat 1), (Code_Numeral.Nat 4)))), uncurry cons (I ((OCL.ST "X\<^sub>P\<^sub>e\<^sub>r\<^sub>s\<^sub>o\<^sub>n3"), I (Ocl_instance_single_ext (SOME ((OCL.SS_base (OCL.ST "X\<^sub>P\<^sub>e\<^sub>r\<^sub>s\<^sub>o\<^sub>n3"))), (OCL.SS_base (OCL.ST "Person")), OclAttrNoCast (nil), ()), Oids ((Code_Numeral.Nat 0), (Code_Numeral.Nat 1), (Code_Numeral.Nat 3)))), uncurry cons (I ((OCL.ST "X\<^sub>P\<^sub>e\<^sub>r\<^sub>s\<^sub>o\<^sub>n2"), I (Ocl_instance_single_ext (SOME ((OCL.SS_base (OCL.ST "X\<^sub>P\<^sub>e\<^sub>r\<^sub>s\<^sub>o\<^sub>n2"))), (OCL.SS_base (OCL.ST "Person")), OclAttrNoCast (uncurry cons (I ((OCL.SS_base (OCL.ST "salary")), ShallB_term (OclDefInteger ((OCL.SS_base (OCL.ST "1800"))))), uncurry cons (I ((OCL.SS_base (OCL.ST "boss")), ShallB_str ((OCL.SS_base (OCL.ST "X\<^sub>P\<^sub>e\<^sub>r\<^sub>s\<^sub>o\<^sub>n2")))), nil))), ()), Oids ((Code_Numeral.Nat 0), (Code_Numeral.Nat 1), (Code_Numeral.Nat 2)))), uncurry cons (I ((OCL.ST "X\<^sub>P\<^sub>e\<^sub>r\<^sub>s\<^sub>o\<^sub>n1"), I (Ocl_instance_single_ext (SOME ((OCL.SS_base (OCL.ST "X\<^sub>P\<^sub>e\<^sub>r\<^sub>s\<^sub>o\<^sub>n1"))), (OCL.SS_base (OCL.ST "Person")), OclAttrNoCast (uncurry cons (I ((OCL.SS_base (OCL.ST "salary")), ShallB_term (OclDefInteger ((OCL.SS_base (OCL.ST "1300"))))), uncurry cons (I ((OCL.SS_base (OCL.ST "boss")), ShallB_str ((OCL.SS_base (OCL.ST "X\<^sub>P\<^sub>e\<^sub>r\<^sub>s\<^sub>o\<^sub>n2")))), nil))), ()), Oids ((Code_Numeral.Nat 0), (Code_Numeral.Nat 1), (Code_Numeral.Nat 1)))), nil))))))))))), nil, true, false, I (uncurry cons ((OCL.ST "dot\<O>\<U>\<T>\<E>\<R>095\<W>\<O>\<R>\<L>\<D>at_pre"), uncurry cons ((OCL.ST "dot\<M>\<O>\<V>\<I>\<N>\<G>at_pre"), uncurry cons ((OCL.ST "dot\<S>\<O>\<U>\<N>\<D>at_pre"), uncurry cons ((OCL.ST "dot\<W>\<E>\<I>\<G>\<H>\<T>at_pre"), uncurry cons ((OCL.ST "dot\<W>\<O>\<R>\<M>\<H>\<O>\<L>\<E>at_pre"), uncurry cons ((OCL.ST "dot\<S>\<A>\<L>\<A>\<R>\<Y>at_pre"), uncurry cons ((OCL.ST "dot_0_\<B>\<O>\<S>\<S>at_pre"), nil))))))), uncurry cons ((OCL.ST "dot\<O>\<U>\<T>\<E>\<R>095\<W>\<O>\<R>\<L>\<D>"), uncurry cons ((OCL.ST "dot\<M>\<O>\<V>\<I>\<N>\<G>"), uncurry cons ((OCL.ST "dot\<S>\<O>\<U>\<N>\<D>"), uncurry cons ((OCL.ST "dot\<W>\<E>\<I>\<G>\<H>\<T>"), uncurry cons ((OCL.ST "dot\<W>\<O>\<R>\<M>\<H>\<O>\<L>\<E>"), uncurry cons ((OCL.ST "dot\<S>\<A>\<L>\<A>\<R>\<Y>"), uncurry cons ((OCL.ST "dot_0_\<B>\<O>\<S>\<S>"), nil)))))))), uncurry cons ((OCL.ST "Sequence_Person"), uncurry cons ((OCL.ST "Set_Person"), uncurry cons ((OCL.ST "Set_Sequence_Planet"), nil))), I (NONE, false), ()) end)))) *}
 Instance \<sigma>\<^sub>1_object0 :: Person = [ "salary" = 1000, "boss" = self 1 ]
      and \<sigma>\<^sub>1_object1 :: Person = [ "salary" = 1200 ]
      and \<sigma>\<^sub>1_object2 :: Person = [ "salary" = 2600, "boss" = X\<^sub>P\<^sub>e\<^sub>r\<^sub>s\<^sub>o\<^sub>n5 ]
      and \<sigma>\<^sub>1_object4 :: Person = [ "salary" = 2300, "boss" = self 2 ]
-Define_state[shallow] \<sigma>\<^sub>1 = [ \<sigma>\<^sub>1_object0, \<sigma>\<^sub>1_object1, \<sigma>\<^sub>1_object2, X\<^sub>P\<^sub>e\<^sub>r\<^sub>s\<^sub>o\<^sub>n5, \<sigma>\<^sub>1_object4, X\<^sub>P\<^sub>e\<^sub>r\<^sub>s\<^sub>o\<^sub>n9 ]
+State[shallow] \<sigma>\<^sub>1 = [ \<sigma>\<^sub>1_object0, \<sigma>\<^sub>1_object1, \<sigma>\<^sub>1_object2, X\<^sub>P\<^sub>e\<^sub>r\<^sub>s\<^sub>o\<^sub>n5, \<sigma>\<^sub>1_object4, X\<^sub>P\<^sub>e\<^sub>r\<^sub>s\<^sub>o\<^sub>n9 ]
 
-(* 136 ************************************ 893 + 1 *)
-Define_state[shallow] \<sigma>\<^sub>1' = [ X\<^sub>P\<^sub>e\<^sub>r\<^sub>s\<^sub>o\<^sub>n1, X\<^sub>P\<^sub>e\<^sub>r\<^sub>s\<^sub>o\<^sub>n2, X\<^sub>P\<^sub>e\<^sub>r\<^sub>s\<^sub>o\<^sub>n3, X\<^sub>P\<^sub>e\<^sub>r\<^sub>s\<^sub>o\<^sub>n4, X\<^sub>P\<^sub>e\<^sub>r\<^sub>s\<^sub>o\<^sub>n6, X\<^sub>P\<^sub>e\<^sub>r\<^sub>s\<^sub>o\<^sub>n7, X\<^sub>P\<^sub>e\<^sub>r\<^sub>s\<^sub>o\<^sub>n8, X\<^sub>P\<^sub>e\<^sub>r\<^sub>s\<^sub>o\<^sub>n9 ]
+(* 136 ************************************ 895 + 1 *)
+State[shallow] \<sigma>\<^sub>1' = [ X\<^sub>P\<^sub>e\<^sub>r\<^sub>s\<^sub>o\<^sub>n1, X\<^sub>P\<^sub>e\<^sub>r\<^sub>s\<^sub>o\<^sub>n2, X\<^sub>P\<^sub>e\<^sub>r\<^sub>s\<^sub>o\<^sub>n3, X\<^sub>P\<^sub>e\<^sub>r\<^sub>s\<^sub>o\<^sub>n4, X\<^sub>P\<^sub>e\<^sub>r\<^sub>s\<^sub>o\<^sub>n6, X\<^sub>P\<^sub>e\<^sub>r\<^sub>s\<^sub>o\<^sub>n7, X\<^sub>P\<^sub>e\<^sub>r\<^sub>s\<^sub>o\<^sub>n8, X\<^sub>P\<^sub>e\<^sub>r\<^sub>s\<^sub>o\<^sub>n9 ]
 
-(* 137 ************************************ 894 + 1 *)
-Define_pre_post[shallow] \<sigma>\<^sub>1 \<sigma>\<^sub>1'
+(* 137 ************************************ 896 + 1 *)
+PrePost[shallow] \<sigma>\<^sub>1 \<sigma>\<^sub>1'
 
-(* 138 ************************************ 895 + 5 *)
+(* 138 ************************************ 897 + 4 *)
 type_synonym Set_Integer = "(\<AA>, Integer\<^sub>b\<^sub>a\<^sub>s\<^sub>e Set\<^sub>b\<^sub>a\<^sub>s\<^sub>e) val"
 consts dot\<C>\<O>\<N>\<T>\<E>\<N>\<T>\<S> :: "Person \<Rightarrow> Set_Integer" ("(_) .contents'(')")
 consts dot\<C>\<O>\<N>\<T>\<E>\<N>\<T>\<S>at_pre :: "Person \<Rightarrow> Set_Integer" ("(_) .contents@pre'(')")
@@ -3300,14 +3368,11 @@ Context[shallow] Person :: contents () : Set(Integer)
                    endif))"
   Post : "(\<lambda> self result. (true))"
   Pre : "(\<lambda> self. (false))"
-thm dot\<C>\<O>\<N>\<T>\<E>\<N>\<T>\<S>_def
 
-(* 139 ************************************ 900 + 2 *)
+(* 139 ************************************ 901 + 1 *)
 Context[shallow] Person   Inv a : "(\<lambda> self. (self .boss <> null implies (self .salary  \<triangleq>  ((self .boss) .salary))))"
-thm Person_aat_pre_def Person_a_def
 
-(* 140 ************************************ 902 + 2 *)
+(* 140 ************************************ 902 + 1 *)
 Context[shallow] Planet   Inv A : "(\<lambda> self. (true and (self .weight \<le>\<^sub>i\<^sub>n\<^sub>t \<zero>)))"
-thm Planet_Aat_pre_def Planet_A_def
 
 end
