doc/Employee_DesignModel_UMLPart_generated.thy
@@ -3340,15 +3340,15 @@ Instance \<sigma>\<^sub>1_object0 :: Person = [ "salary" = 1000, "boss" = self 1
      and \<sigma>\<^sub>1_object1 :: Person = [ "salary" = 1200 ]
      and \<sigma>\<^sub>1_object2 :: Person = [ "salary" = 2600, "boss" = X\<^sub>P\<^sub>e\<^sub>r\<^sub>s\<^sub>o\<^sub>n5 ]
      and \<sigma>\<^sub>1_object4 :: Person = [ "salary" = 2300, "boss" = self 2 ]
-Define_state[shallow] \<sigma>\<^sub>1 = [ \<sigma>\<^sub>1_object0, \<sigma>\<^sub>1_object1, \<sigma>\<^sub>1_object2, X\<^sub>P\<^sub>e\<^sub>r\<^sub>s\<^sub>o\<^sub>n5, \<sigma>\<^sub>1_object4, X\<^sub>P\<^sub>e\<^sub>r\<^sub>s\<^sub>o\<^sub>n9 ]
+State[shallow] \<sigma>\<^sub>1 = [ \<sigma>\<^sub>1_object0, \<sigma>\<^sub>1_object1, \<sigma>\<^sub>1_object2, X\<^sub>P\<^sub>e\<^sub>r\<^sub>s\<^sub>o\<^sub>n5, \<sigma>\<^sub>1_object4, X\<^sub>P\<^sub>e\<^sub>r\<^sub>s\<^sub>o\<^sub>n9 ]
 
 (* 136 ************************************ 895 + 1 *)
-Define_state[shallow] \<sigma>\<^sub>1' = [ X\<^sub>P\<^sub>e\<^sub>r\<^sub>s\<^sub>o\<^sub>n1, X\<^sub>P\<^sub>e\<^sub>r\<^sub>s\<^sub>o\<^sub>n2, X\<^sub>P\<^sub>e\<^sub>r\<^sub>s\<^sub>o\<^sub>n3, X\<^sub>P\<^sub>e\<^sub>r\<^sub>s\<^sub>o\<^sub>n4, X\<^sub>P\<^sub>e\<^sub>r\<^sub>s\<^sub>o\<^sub>n6, X\<^sub>P\<^sub>e\<^sub>r\<^sub>s\<^sub>o\<^sub>n7, X\<^sub>P\<^sub>e\<^sub>r\<^sub>s\<^sub>o\<^sub>n8, X\<^sub>P\<^sub>e\<^sub>r\<^sub>s\<^sub>o\<^sub>n9 ]
+State[shallow] \<sigma>\<^sub>1' = [ X\<^sub>P\<^sub>e\<^sub>r\<^sub>s\<^sub>o\<^sub>n1, X\<^sub>P\<^sub>e\<^sub>r\<^sub>s\<^sub>o\<^sub>n2, X\<^sub>P\<^sub>e\<^sub>r\<^sub>s\<^sub>o\<^sub>n3, X\<^sub>P\<^sub>e\<^sub>r\<^sub>s\<^sub>o\<^sub>n4, X\<^sub>P\<^sub>e\<^sub>r\<^sub>s\<^sub>o\<^sub>n6, X\<^sub>P\<^sub>e\<^sub>r\<^sub>s\<^sub>o\<^sub>n7, X\<^sub>P\<^sub>e\<^sub>r\<^sub>s\<^sub>o\<^sub>n8, X\<^sub>P\<^sub>e\<^sub>r\<^sub>s\<^sub>o\<^sub>n9 ]
 
 (* 137 ************************************ 896 + 1 *)
-Define_pre_post[shallow] \<sigma>\<^sub>1 \<sigma>\<^sub>1'
+PrePost[shallow] \<sigma>\<^sub>1 \<sigma>\<^sub>1'
 
-(* 138 ************************************ 897 + 5 *)
+(* 138 ************************************ 897 + 4 *)
 type_synonym Set_Integer = "(\<AA>, Integer\<^sub>b\<^sub>a\<^sub>s\<^sub>e Set\<^sub>b\<^sub>a\<^sub>s\<^sub>e) val"
 consts dot\<C>\<O>\<N>\<T>\<E>\<N>\<T>\<S> :: "Person \<Rightarrow> Set_Integer" ("(_) .contents'(')")
 consts dot\<C>\<O>\<N>\<T>\<E>\<N>\<T>\<S>at_pre :: "Person \<Rightarrow> Set_Integer" ("(_) .contents@pre'(')")
@@ -3359,14 +3359,11 @@ Context[shallow] Person :: contents () : Set(Integer)
                    endif))"
   Post : "(\<lambda> self result. (true))"
   Pre : "(\<lambda> self. (false))"
-thm dot\<C>\<O>\<N>\<T>\<E>\<N>\<T>\<S>_def
 
-(* 139 ************************************ 902 + 2 *)
+(* 139 ************************************ 901 + 1 *)
 Context[shallow] Person   Inv a : "(\<lambda> self. (self .boss <> null implies (self .salary  \<triangleq>  ((self .boss) .salary))))"
-thm Person_aat_pre_def Person_a_def
 
-(* 140 ************************************ 904 + 2 *)
+(* 140 ************************************ 902 + 1 *)
 Context[shallow] Planet   Inv A : "(\<lambda> self. (true and (self .weight \<le>\<^sub>i\<^sub>n\<^sub>t \<zero>)))"
-thm Planet_Aat_pre_def Planet_A_def
 
 end
